# Differentiation

*automatic and symbolic differentiation is a key building block for scientific computing software*

The backbone of any numerical/scientific/machine learning software is
an automatic and/or symbolic differentiation. In SciLean, automatic and
symbolic differentiation is build on top of these two operators:

1. Differential `∂ : (X → Y) → (X → X → Y)`

2. Adjoint `†: (X → Y) → (Y → X)`

The differential `∂` tells us how much does the function `f : X → Y`
changes in the direction `dx : X` at the point `x : X`. The usual
mathematical definition is:

\(
  \partial \texttt{f x dx} := \lim_{h \rightarrow 0} \frac{f(x + dx) - f(x)}{h}
\)


`$$ \frac{1}{3} $$`

Because mathlib is not yet ported to Lean 4 this definition is not used
in SciLean. Right now, the differential `∂` is just postulated to exist.


The adjoint `†` is just well known matrix transposition. Thus for real
valued matrix `A`

.. math:: (A^\dagger)_{ij} = A_{ji}

..

For a general linear map `A : X → Y` between two Hilbert spaces `X` and `Y`,
the adjoint is defined via

.. math :: \langle A x, y \rangle = \langle x, A^\dagger y \rangle  \qquad \, \forall x \in X, \,y \in Y

-/

/-!

We will show that these two operators give a rise to a whole zoo of operators

1. Differential `∂ : (X → Y) → (X → X → Y)`

2. Adjoint `†: (X → Y) → (Y → X)`

3. Adjoint Differential `∂† : (X → Y) → (X → Y → X)`

4. Derivative `ⅆ : (ℝ → X) → (ℝ → X)`

5. Gradient `∇ : (X → ℝ) → (X → X)`

6. Divergence `∇· : (X → X) → (X → ℝ)`

7. Forward Mode AD `fwdDiff : (X → Y) → (X → X×(X → Y))`

8. Reverse Mode AD `revDiff : (X → Y) → (X → X×(Y → X))`

9. Dual Number AD `dualDiff : (X → Y) → (X×X → Y×Y)`

 -/

/-!

Differential
============

 -/

section Differential

/-!

The simples possible example: What is the differential of identity function?

 -/

  #check (∂ λ x : ℝ => x)
    rewrite_by (simp; trace_state /- .unfold -/ )

/-!

As expected the change of identity function is just `dx` and it does not depend
on the position `x`.


(Note: The SciLean's custom notation `x:term rewrite_by t:convSeq`
applies tactic `t` on the term `x`. This notation confuses the `#check`
command. To see the actual result it is better to use the `trace_state`
tactic. TODO: Add a document explaining the technical detail of `rewrite_by`
notation. TODO: Add delaborator for terms created with `AutoImpl`)

Another way to check that the differential is computed correctly

 -/

 example : (∂ λ x : ℝ => x) = (λ x dx => dx) := by simp

/-!

This has the disadvantages that we need to know the result beforehand.


Few more basic derivatives: of a constant, quadratic function, sine

 -/

  #check (∂ λ x : ℝ => (1 : ℝ))
    rewrite_by
    (simp; trace_state) /- .unfold -/

  #check (∂ λ x : ℝ => x * x)
    rewrite_by
    (simp; trace_state) /- .unfold -/

  #check (∂ λ x : ℝ => Math.sin x)
    rewrite_by
    (simp; trace_state) /- .unfold -/


/-!

The result `fun x dx => dx * x + x * dx` is slightly undesirable. We
would like to get `fun x dx => 2 * dx * x`. Such algebraic manipulation
is within the scope of mathlib's tactics so we will wait for mathlib
port to Lean 4.

 -/

/-!

Let's introduce few generic functions  to demonstrate some general differentiation
results

 -/
  variable {X Y Z : Type} [Vec X] [Vec Y] [Vec Z]
  variable (f : Y → Z) [IsSmooth f]
  variable (g : X → Y) [IsSmooth g]

/-!

The most crucial tool when computing derivatives is the chain rule, as a proof

 -/

  example : (∂ λ x => f (g x)) = (λ x dx => ∂ f (g x) (∂ g x dx)) :=
    by simp

/-!

Or as a symbolic computation

 -/

  #check (∂ λ x => f (g x))
    rewrite_by
    (simp; trace_state) /- .unfold -/


/-!

Another common rule is the product rule

 -/

  variable (ϕ ψ : ℝ → ℝ) [IsSmooth ϕ] [IsSmooth ψ]

  #check (∂ λ x => ϕ x * ψ x)
    rewrite_by
    (simp; trace_state) /- .unfold -/

/-!

Derivative
----------

The standard notion of derivative takes a function from reals to reals, `f : ℝ → ℝ`,
and produces again a function from, usually denoted with `f' : ℝ → ℝ`.

The differential `∂` does not fit this. The well know result that
derivative of exponential is exponential `exp' = exp` can't be expressed as
easily with differential.

The naive statement does not even typecheck

 -/

  #check_failure ∂ Math.exp = Math.exp

/-!

The `exp' = exp` is this slightly cumbersome statement

 -/

  example : (λ t => ∂ Math.exp t 1) = Math.exp := by simp

/-!

For this reason we introduce a new operator, derivative `ⅆ : (ℝ → X) → (ℝ → X)`.
Which is defines as follows

 -/

  example (f : ℝ → X) : ⅆ f = λ t => ∂ f t 1 :=
    by simp

/-!

Now we have

 -/

  example : ⅆ Math.exp = Math.exp := by simp

/-!

(TODO: Right now simplifier needs to unfold `derivative`. Fix it!)

We provide convenient notation, `ⅆ t, f t` and `ⅆ (t:=t₀), f t`, for
taking derivative with a respect to an explicit variable.

 -/
  section DerivativeNotation

    variable (f : ℝ → X) (t₀ : ℝ)

    -- effectively translates `t,` to `λ t =>`
    example : (ⅆ t, f t) = ⅆ (λ t => f t ) := by rfl

    -- similar as above but also applies `t₀`
    example : (ⅆ (t:=t₀), f t) = ⅆ (λ t => f t) t₀ := by rfl

  end DerivativeNotation

/-!

..

The notation `ⅆ (t:=t₀), f t` tries to mimic the mathematical notation

.. math:: \frac{d}{dt}\bigg\rvert_{t=t_0} f(t)

 -/

/-!

Debugging Differentiation
-------------------------

Sometimes the differentiation is not doing what we expect. It is crucial
to know how to figure out what went wrong.

To demonstrate this, let's introduce a function `h` but without the smoothness
proof i.e. we do not introduce `[IsSmooth h]`

 -/

  variable (h : X → Y)

/-!

Now the chain rule for `f` and `h` fails

 -/

  example : (∂ λ x => f (h x)) = (λ x dx => ∂ f (h x) (∂ h x dx)) :=
    by simp   -- no progress
       admit  -- we have to give up

/-!

We have to use the `admit` tactic to close the goal as `simp` is unable
to do it right now.

The problem is that `simp` can't apply chain rule because it is missing
the proof of smoothness of `h`. To figure this out, we turn on the option
`trace.Meta.Tactic.simp.discharge`

 -/

  set_option trace.Meta.Tactic.simp.discharge true in
  example : (∂ λ x => f (h x)) = (λ x dx => ∂ f (h x) (∂ h x dx)) :=
    by simp; admit

/-!

If you click on `simp`, one of the messages will be

::

  [Meta.Tactic.simp.discharge] SciLean.diff_of_comp, failed to synthesize instance
      SciLean.IsSmooth fun x => h x

(TODO: currently there is tons of crap that should not be there)

If we provide the smoothness proof we can observe all rewrites by turning on
`trace.Meta.Tactic.simp.rewrite`

-/

  variable [IsSmooth h]

  set_option trace.Meta.Tactic.simp.rewrite true in
  example : (∂ λ x => f (h x)) = (λ x dx => ∂ f (h x) (∂ h x dx)) :=
    by simp

/-!

Now `simp` shows the application of the chain rule

::

  [Meta.Tactic.simp.rewrite] SciLean.diff_of_comp:99, ∂fun x =>
        f (h x) ==> fun x dx => SciLean.differential f (h x) (SciLean.differential (fun x => h x) x dx)


A bit more complicated computation

 -/

  set_option trace.Meta.Tactic.simp.rewrite true in
  #check (∂ λ x : ℝ => x * Math.exp (x*x) + x)
    rewrite_by
    (simp; trace_state) /- .unfold -/

/-!

Clicking on `simp` reveals fairly long list of rewrites.

 -/

end Differential



/-!

Defining Differentiable Function
================================

Sometimes we want to define our own differentiable functions

 -/

def square (x : ℝ) := x * x

/-!

We might be surprized that differentiating this function does not work

 -/

example : (∂ square) = (λ x dx => dx * x + x * dx) :=
by
  simp  -- this does nothing as we know nothing about `square`
  unfold square  -- unfold definition of `square`
  simp  -- now it works

/-!

Manually unfolding every definition can get tedious. To circumvent that,
we can annotate the definition of `square` to indicate that it is
differentiable.

 -/

def square_v1 (x : ℝ) : ℝ := x * x
argument x
  isSmooth, diff

/-!

(TODO: When using `def` with annotations, we **have to** explicitly specify
the return type. Remove this limitation or add a warning when the
return type is missing.)

The `argument x` specifies that everything that follows concerns the
argument `x`. The `isSmooth` generates proof that `square_v1` is
smooth in the argument `x` and `diff` defines a new function
`square_v1.arg_x.diff` that is the function's differential.

There are few variants that are useful when full automation fails or
produces undesirable results.

 -/

def square_v2 (x : ℝ) : ℝ := x * x
argument x
  -- specify how to prove smoothness
  isSmooth := by unfold square_v2; infer_instance,
  -- specify what the differential is and how to prove it
  diff := 2 * dx * x by simp[diff, square_v2]; funext x dx; ring

def square_v3 (x : ℝ) : ℝ := x * x
argument x
  -- proof is done automatically
  isSmooth,
  -- specify how to compute differential
  diff by simp[square_v3]

/-!

Defining a new function, `square_v1.arg_x.diff` for the differential
can be undesirable. Sometimes we want `∂ square` to directly simplify
to `λ x dx => dx * x + x * dx`. To achieve this, we use `diff_simp`
instead of `diff`.

 -/

def square_v4 (x : ℝ) : ℝ := x * x
argument x
  isSmooth,
  diff_simp by simp[square_v4]

/-!

The `diff_simp` annotation allows the same variants as `diff`.

Proof that the second derivative is `2`. We have to do manual unfolding
when working with `square_v3` but with `square_v4` the proof is immediate

 -/

example : (λ x => ∂ ∂ square_v2 x 1 1) = (λ x => 2) :=
by
  simp  -- simp gets stopped on `square_v3.arg_x.diff`
  unfold square_v2.arg_x.diff -- manually unfold definition
  simp  -- we can continue with computation

example : (λ x => ∂ ∂ square_v4 x 1 1) = (λ x => 2) :=
by
  simp  -- done immediately

/-!

We missed our chance to add annotations to the original function `square`.
We can add additional annotations later on with `function_properties`.

-/

function_properties square (x : ℝ) : ℝ
argument x
  isSmooth, diff_simp

-- now we can differentiate `square`
example : ∂ square = λ x dx => dx * x + x * dx := by simp

/-!

The keyword `function_properties` works exactly like `def` with annotations
but you do not provide the function definition `:= ...`. Argument types
and order have to match exactly the original definition but the argument
names do not have to be the same.

 -/

/-!

Multiple Arguments
------------------

(TODO: Explain how annotations work with multiple arguments. The current
behavior is a bit limiting, so I should rewrite how they work before
I write this section.)

 -/

/-!

How Do Annotations Work?
------------------------

The `isSmooth` and `diff` annotations might appear mysterious but they
are simple macros.

This definition
 -/

def cube (x : ℝ) : ℝ := x * x * x
argument x
  isSmooth := by unfold cube; infer_instance,
  diff := 3 * dx * x * x by simp[diff,cube]; funext x dx; ring

/-!

Is unfolded to (we have to use a new identifier `cube_v1` as `cube` is
already defined)

 -/

def cube_v1 (x : ℝ) : ℝ := x * x * x

-- proof of smoothness
instance cube_v1.arg_x.isSmooth : IsSmooth (λ x => cube_v1 x) :=
by unfold cube_v1; infer_instance

-- differential definition
def cube_v1.arg_x.diff (x dx : ℝ) : ℝ := 3 * dx * x * x

-- simplifier rule
@[simp]
theorem cube_v1.arg_x.diff_simp
  : ∂ cube_v1 = cube_v1.arg_x.diff :=
by simp[diff,cube_v1]; funext x dx; ring

/-!

Using `diff_simp` annotation does not define `cube_v1.arg_x.diff` and
the simp theorem states directly `∂ cube_v1 = λ x dx => 3 * dx * x * x`.

 -/

/-!

Adjoint Differential
====================

Finding the minimum of a function `f : X → ℝ` with gradient descent
requires function's gradient `∇ f : X → X`.

However, can we compute the gradient just with the differential `∂`?
No we can't! We need an adjoint `†` too!

The differential `∂ f x` at point `x` is a linear function `X → R`.
When we take an adjoint and apply one we get an element of `X`. That
is the gradient of `f` at `x`!

In finite dimension, we can think about differential `∂ f x` is a row vector.
To get a column vector we have to transpose it i.e. take its adjoint.

For general function `f : X → Y`, we define adjoint differential
`∂† : (X → Y) → (X → Y → X)` as `∂† f x dy := (∂ f x)† dy`

Taking adjoint makes sense only for functions between Hilbert spaces.
Let's introduce few of those

 -/

section AdjointDifferential

  variable {X Y Z} [Hilbert X] [Hilbert Y] [Hilbert Z]

/-!

To stress the definition of adjoint differential

 -/

  example (f : X → Y) : ∂† f = λ x dy => (∂ f x)† dy := by rfl

/-!

Similarly to derivative `ⅆ`, we define a specialized operator gradient `∇`
for real valued functions over any Hilbert space

 -/

  example (f : X → ℝ) : ∇ f = λ x => (∂ f x)† 1 := by rfl

/-!

The important result is that the gradient of squared norm `∥x∥²` is `2*x`

 -/


  #check (∇ (x : X), ∥x∥²)
    rewrite_by
    (simp; trace_state)  /- .unfold -/

/-!

(TODO: Make sure we do not need to unfold gradient and hold here`)

Another fun result is that the gradient of `⟪A x, x⟫` is `(A† + A) x`

 -/

  variable (A : X → X) [HasAdjDiff A] [IsLin A]

  #check (∇ x, ⟪A x, x⟫)
    rewrite_by
    (simp[adjointDifferential]; trace_state) /- .unfold -/

/-!

(TODO: Ughh, this requires too many assumptions on A and too many unfolding`)

Similar to chain rule for differential, we have a chain rule for the adjoint
differential but the composition is in reverse

 -/

  variable (f : Y → Z) [HasAdjDiff f]
  variable (g : X → Y) [HasAdjDiff g]

  example : (∂† λ x => f (g x)) = (λ x dz => ∂† g x (∂† f (g x) dz)) :=
    by simp

/-!

(TODO: Explain what `HasAdjDiff f` is)

 -/


/-!

Euler-Lagrange Equations
------------------------

Let's write down Euler-Lagrange equations to demonstrate SciLean's notation
in a bit complicated scenario.

They are usually written in the following way

.. math:: \frac{d}{dt} \frac{\partial}{\partial \dot x} L(x(t),\dot x(t)) - \frac{\partial}{\partial x} L(x(t),\dot x(t)) = 0

However, the partial derivative notation is really ambiguous. Thus a bit
more explicit form is

.. math:: \frac{d}{ds}\bigg\rvert_{s=t} \frac{\partial}{\partial v}\bigg\rvert_{v=\dot y(s)} L(y(s),v) - \frac{\partial}{\partial x}\bigg\rvert_{x=y(t)} L(x, \dot y(t)) = 0

And this form can be written in SciLean relatively nicely.

 -/

  variable (L : X → X → ℝ)  -- Lagrangian
  variable (y : ℝ → X)      -- trajectory
  variable (t : ℝ)          -- time

  #check
    ⅆ (s:=t), ∇ (v:=ⅆ y s), L (y s) v - ∇ (x:=y t), L x (ⅆ y t) = 0

/-!

Let's plug in a Lagrangian for a particle in a potential field and hopefully
we get the correct equations of motion.

 -/
  def L' (ϕ : X → ℝ) (m : ℝ) (x v : X) := 1/2*m*∥v∥² - ϕ x

  variable [IsSmooth y]  -- trajectory is smooth
  variable (ϕ : X → ℝ)  [HasAdjDiff ϕ]
  variable (m : ℝ) -- mass

  #check
    (ⅆ (s:=t), ∇ (v:=ⅆ y s), L' ϕ m (y s) v
     -
     ∇ (x:=y t), L' ϕ m x (ⅆ y t))
    rewrite_by
    (-- Currently broken :(
     -- simp
     -- simp[gradient,hold]
     -- simp[derivative]
     trace_state) /- .unfold -/

/-!

(TODO: Make sure we get these rewrite to make the result look nicer

  `2 * (1/2) = 1`

  `differential (∂y) t 1 1 = ⅆ (ⅆ y) t`

  `adjointDifferential (fun x => ϕ x) (y t) (-1) = - ∇ ϕ (y t)`)

The result is (with the TODO rewrites) `m * ⅆ (ⅆ y) t + ∇ ϕ (y t)` which
exactly corresponds to the equation of a particle in a potential field `ϕ`

.. math:: m \ddot y(t) = - \nabla \phi (y(t))

 -/

end AdjointDifferential
